src/DY.Lib.State.Typed.fst
@@ -48,10 +48,10 @@ let typed_session_pred_to_session_pred #cinvs #a #ps_a tspred =
 
 val has_typed_session_pred:
   #a:Type -> {|parseable_serializeable bytes a|} ->
-  invs:protocol_invariants -> string -> typed_session_pred a ->
+  invs:protocol_invariants -> (string & typed_session_pred a) ->
   prop
-let has_typed_session_pred #a #ps_a invs label spred =
-  has_session_pred invs label (typed_session_pred_to_session_pred spred)
+let has_typed_session_pred #a #ps_a invs (label, spred) =
+  has_session_pred invs (label, (typed_session_pred_to_session_pred spred))
 
 [@@ "opaque_to_smt"]
 val typed_state_was_set:
@@ -87,7 +87,7 @@ val set_typed_state_invariant:
   (requires
     spred.pred tr prin sess_id content /\
     trace_invariant tr /\
-    has_typed_session_pred invs label spred
+    has_typed_session_pred invs (label, spred)
   )
   (ensures (
     let ((), tr_out) = set_typed_state label prin sess_id content tr in
@@ -96,7 +96,7 @@ val set_typed_state_invariant:
   ))
   [SMTPat (set_typed_state label prin sess_id content tr);
    SMTPat (trace_invariant tr);
-   SMTPat (has_typed_session_pred invs label spred)]
+   SMTPat (has_typed_session_pred invs (label, spred))]
 let set_typed_state_invariant #a #ps_a #invs label spred prin sess_id content tr =
   reveal_opaque (`%set_typed_state) (set_typed_state #a);
   reveal_opaque (`%typed_state_was_set) (typed_state_was_set #a);
@@ -110,7 +110,7 @@ val get_typed_state_invariant:
   Lemma
   (requires
     trace_invariant tr /\
-    has_typed_session_pred invs label spred
+    has_typed_session_pred invs (label, spred)
   )
   (ensures (
     let (opt_content, tr_out) = get_typed_state label prin sess_id tr in
@@ -124,7 +124,7 @@ val get_typed_state_invariant:
   ))
   [SMTPat (get_typed_state #a label prin sess_id tr);
    SMTPat (trace_invariant tr);
-   SMTPat (has_typed_session_pred invs label spred)]
+   SMTPat (has_typed_session_pred invs (label, spred))]
 let get_typed_state_invariant #a #ps_a #invs label spred prin sess_id tr =
   reveal_opaque (`%get_typed_state) (get_typed_state #a)
 
@@ -137,12 +137,12 @@ val typed_state_was_set_implies_pred:
   (requires
     typed_state_was_set tr label prin sess_id content /\
     trace_invariant tr /\
-    has_typed_session_pred invs label spred
+    has_typed_session_pred invs (label, spred)
   )
   (ensures spred.pred tr prin sess_id content)
   [SMTPat (typed_state_was_set tr label prin sess_id content);
    SMTPat (trace_invariant tr);
-   SMTPat (has_typed_session_pred invs label spred);
+   SMTPat (has_typed_session_pred invs (label, spred));
   ]
 let typed_state_was_set_implies_pred #a #ps_a invs tr label spred prin sess_id content =
   parse_serialize_inv_lemma #bytes a content;
